theories/logatom/conditional_increment/spec.v
@@ -1,14 +1,14 @@
 From stdpp Require Import namespaces.
 From iris.heap_lang Require Export lifting notation.
 From iris.program_logic Require Export atomic.
+From iris_examples.logatom.lib Require Export gc.
 Set Default Proof Using "Type".
 
 (** A general logically atomic interface for conditional increment. *)
-Record atomic_cinc {Σ} `{!heapG Σ} := AtomicCinc {
+Record atomic_cinc {Σ} `{!heapG Σ, !gcG Σ} := AtomicCinc {
   (* -- operations -- *)
   new_counter : val;
   cinc : val;
-  set_flag : val;
   get : val;
   (* -- other data -- *)
   name : Type;
@@ -16,34 +16,31 @@ Record atomic_cinc {Σ} `{!heapG Σ} := AtomicCinc {
   name_countable : Countable name;
   (* -- predicates -- *)
   is_counter (N : namespace) (γs : name) (v : val) : iProp Σ;
-  counter_content (γs : name) (flag : bool) (c : Z) : iProp Σ;
+  counter_content (γs : name) (c : Z) : iProp Σ;
   (* -- predicate properties -- *)
   is_counter_persistent N γs v : Persistent (is_counter N γs v);
-  counter_content_timeless γs f c : Timeless (counter_content γs f c);
-  counter_content_exclusive γs f1 c1 f2 c2 :
-    counter_content γs f1 c1 -∗ counter_content γs f2 c2 -∗ False;
+  counter_content_timeless γs c : Timeless (counter_content γs c);
+  counter_content_exclusive γs  c1 c2 :
+    counter_content γs c1 -∗ counter_content γs c2 -∗ False;
   (* -- operation specs -- *)
   new_counter_spec N :
+    N ## gcN →
+    gc_inv -∗
     {{{ True }}}
         new_counter #()
-    {{{ ctr γs, RET ctr ; is_counter N γs ctr ∗ counter_content γs true 0 }}};
-  cinc_spec N γs v :
+    {{{ ctr γs, RET ctr ; is_counter N γs ctr ∗ counter_content γs 0 }}};
+  cinc_spec N γs v (f : loc) :
     is_counter N γs v -∗
-    <<< ∀ (b : bool) (n : Z), counter_content γs b n >>>
-        cinc v @⊤∖↑N
-    <<< counter_content γs b (if b then n + 1 else n), RET #() >>>;
-  set_flag_spec N γs v (new_b: bool) :
-    is_counter N γs v -∗
-    <<< ∀ (b : bool) (n : Z), counter_content γs b n >>>
-        set_flag v #new_b @⊤∖↑N
-    <<< counter_content γs new_b n, RET #() >>>;
+    <<< ∀ (b : bool) (n : Z), counter_content γs n ∗ gc_mapsto f #b >>>
+        cinc v #f @⊤∖↑N∖↑gcN
+    <<< counter_content γs (if b then n + 1 else n) ∗ gc_mapsto f #b, RET #() >>>;
   get_spec N γs v:
     is_counter N γs v -∗
-    <<< ∀ (b : bool) (n : Z), counter_content γs b n >>>
-        get v @⊤∖↑N
-    <<< counter_content γs b n, RET #n >>>;
+    <<< ∀ (n : Z), counter_content γs n >>>
+        get v @⊤∖↑N∖↑gcN
+    <<< counter_content γs n, RET #n >>>;
 }.
-Arguments atomic_cinc _ {_}.
+Arguments atomic_cinc _ {_ _}.
 
 Existing Instances
   is_counter_persistent counter_content_timeless
